### 3.3 Differentiation Rules


- ðŸŽ¯ geogebra practice 

```
# EXAMPLE 3.22

f(x)=x^(2)-4 x+6
f'(x)=Derivative(f(x))
A=(1,f(1))
m=f'(1)
g: y=f'(1) (x-x(A))+y(A)
```


- ðŸŽ¯ geogebra practice 

```
# EXAMPLE 3.24

f(x)=x^(2)+2
g(x)=3 x^(3)-5 x
h(x)=f(x) g(x)
k(x)=Expand(h(x))
f'_{1}(x)=Derivative(f(x)) g(x)+Derivative(g(x)) f(x)
p(x)=Expand(f'_{1}(x))
q(x)=Derivative(k(x))
```


- ðŸŽ¯ geogebra practice 

```
# EXAMPLE 3.25

f(x)=5 x^(2)
g(x)=4 x+3
k(x)=((f(x))/(g(x)))
k'(x)=Derivative(k(x))
h(x)=((Derivative(f(x)) g(x)-Derivative(g(x)) f(x))/((g(x))^(2)))
p(x)=Expand(h(x))
```


- ðŸŽ¯ geogebra practice 

```
# EXAMPLE 3.31

f(x)=x^(3)-7 x^(2)+8 x+1
f'(x)=Derivative(f(x))
l1=Solve(f'(x))
```


- ðŸŽ¯ geogebra practice 

```
# EXAMPLE 3.32

s(t)=((t)/(t^(2)+1))
v(t)=Derivative(s(t))
v_{0}=v(0)
```





